Core/Eval/SmallStep.lean
@@ -17,11 +17,11 @@ def inline_insts (n : String) (G : List Global) (sp : List SpineElem) :=
 
 @[simp]
 def eval_choice_mapping (G : List Global) : Term -> Option Term
-| .match (.ctor2 .choice t1 t2) ps ts c =>
-  return (.match t1 ps ts c `+ .match t2 ps ts c)
-| .match s ps ts c => do
+| .match n (.ctor2 .choice t1 t2) ps ts c =>
+  return (.match n t1 ps ts c `+ .match n t2 ps ts c)
+| .match n s ps ts c => do
   let s' <- eval_choice_mapping G s
-  return .match s' ps ts c
+  return .match n s' ps ts c
 
 | .guard  p (.ctor2 .choice s1 s2) t =>
   return (.guard p s1 t `+ .guard p s2 t)
@@ -68,10 +68,10 @@ def eval_choice_mapping (G : List Global) : Term -> Option Term
 
 @[simp]
 def eval_const_folding_zero (G : List Global) : Term -> Option Term
-| .match `0 _ _ _=> return `0
-| .match s ps ts c => do
+| .match n `0 _ _ _=> return `0
+| .match n s ps ts c => do
   let s' <- eval_const_folding_zero G s
-  return .match s' ps ts c
+  return .match n s' ps ts c
 | .guard _ `0 _ => return `0
 | .guard p s t => do
   let s' <- eval_const_folding_zero G s
@@ -116,9 +116,9 @@ def eval_const_folding_zero (G : List Global) : Term -> Option Term
 
 @[simp]
 def eval_const_folding_refl (G : List Global) : Term -> Option Term
-| .match s ps ts c => do
+| .match n s ps ts c => do
   let s' <- eval_const_folding_refl G s
-  return .match s' ps ts c
+  return .match n s' ps ts c
 | .guard p s t => do
   let s' <- eval_const_folding_refl G s
   return .guard p s' t
@@ -203,7 +203,7 @@ def eval_inst_beta (G : List Global) :  Term -> Option Term
    let p_pats : Vect n String := λ i => (ps i).1
    let p_sps : Vect n (List SpineElem) := λ i => (ps i).2
    match eval_inst_beta G s with
-   | .some s' => return .match s' ps' cs default
+   | .some s' => return .match n s' ps' cs default
    | .none => match s.spine with
            | .none => .none -- stuck term, cannot evaluate and not in neutral form
            | .some (s_x, s_sp) => do
